feat: make remaining definitions universe polymorphic

CTree/LTSInf.lean
@@ -6,7 +6,7 @@ namespace CTree
     Labelled transition system for `CTree`s.
   -/
 
-  inductive StateInf (ε : Type → Type) (ρ : Type)
+  inductive StateInf ε ρ
   | ct : CTree ε ρ → StateInf ε ρ
   | kt {α} : KTree ε α ρ → StateInf ε ρ
   | div : StateInf ε ρ
@@ -15,12 +15,12 @@ namespace CTree
   notation:150 "K∞[ " t " ]" => StateInf.kt t
   notation:151 "K∞[ " α' " | " t " ]" => StateInf.kt (α := α') t
 
-  inductive DivergeF {ε : Type → Type} {ρ : Type} (sim : CTree ε ρ → Prop) : CTree ε ρ → Prop
+  inductive DivergeF (sim : CTree ε ρ → Prop) : CTree ε ρ → Prop
     | tau {t : CTree ε ρ} : sim t → DivergeF sim t.tau
     | choice_left {c1 c2 : CTree ε ρ} : sim c1 → DivergeF sim (c1 ⊕ c2)
     | choice_right {c1 c2 : CTree ε ρ} : sim c2 → DivergeF sim (c1 ⊕ c2)
 
-  theorem DivergeF.monotone {ε : Type → Type} {ρ : Type} {t : CTree ε ρ}
+  theorem DivergeF.monotone {t : CTree ε ρ}
     (sim1 sim2 : CTree ε ρ → Prop) (hsim : ∀ t, sim1 t → sim2 t) (h : DivergeF sim1 t) : DivergeF sim2 t := by
     cases h with
     | tau h => exact .tau (hsim _ h)
@@ -30,19 +30,19 @@ namespace CTree
   /--
     Whether a `CTree` can silenty diverge
   -/
-  def Diverge {ε : Type → Type} {ρ : Type} (t : CTree ε ρ) : Prop :=
+  def Diverge (t : CTree ε ρ) : Prop :=
     DivergeF Diverge t
     coinductive_fixpoint monotonicity by
       intro _ _ hsim _ h
       exact DivergeF.monotone _ _ hsim h
 
-  inductive Label (ε : Type → Type) (ρ : Type)
+  inductive Label (ε : Type u → Type v) (ρ : Type w)
   | val (v : ρ)
-  | event (α : Type) (e : ε α)
-  | response (α : Type) (a : α)
+  | event (α : Type u) (e : ε α)
+  | response (α : Type u) (a : α)
   | div
 
-  inductive Step {ε ρ} : StateInf ε ρ → Label ε ρ → StateInf ε ρ → Prop
+  inductive Step : StateInf ε ρ → Label ε ρ → StateInf ε ρ → Prop
   | ret {v : ρ} : Step (C∞[ @ret ε ρ v ]) (.val v) (C∞[ zero ])
   | event {α} {e : ε α} {k : α → CTree ε ρ}
     : Step (C∞[ vis e k ]) (.event α e) (K∞[ k ])
@@ -56,7 +56,7 @@ namespace CTree
     : Step (C∞[ t2 ]) l t3 → Step (C∞[ t1 ⊕ t2 ]) l t3
   | div {t : CTree ε ρ} : Diverge t → Step (C∞[ t ]) .div .div
 
-  def IsSimulation {ε : Type → Type} {ρ : Type} (sim : Rel (StateInf ε ρ) (StateInf ε ρ)) : Prop :=
+  def IsSimulation (sim : Rel (StateInf ε ρ) (StateInf ε ρ)) : Prop :=
     ∀ p1 q1, sim p1 q1 →
       match p1, q1 with
       | C∞[ _ ], C∞[ _ ] =>
@@ -66,13 +66,13 @@ namespace CTree
       | .div, .div => True
       | _, _ => False
 
-  def IsBisimulation {ε : Type → Type} {ρ : Type} (sim : Rel (StateInf ε ρ) (StateInf ε ρ)) : Prop :=
+  def IsBisimulation (sim : Rel (StateInf ε ρ) (StateInf ε ρ)) : Prop :=
     IsSimulation sim ∧ IsSimulation (flip sim)
 
-  def Sim {ε : Type → Type} {ρ : Type} : Rel (StateInf ε ρ) (StateInf ε ρ) :=
+  def Sim : Rel (StateInf ε ρ) (StateInf ε ρ) :=
     λ p q => ∃ sim, IsSimulation sim ∧ sim p q
 
-  def Bisim {ε : Type → Type} {ρ : Type} : Rel (StateInf ε ρ) (StateInf ε ρ) :=
+  def Bisim : Rel (StateInf ε ρ) (StateInf ε ρ) :=
     λ p q => ∃ sim, IsBisimulation sim ∧ sim p q
 
   theorem infTau_diverge : Diverge (@infTau ε ρ) := by
